theories/MaxOfTwoNumbersSimpler/Computed/logit_delta.v
@@ -1,0 +1,12 @@
+From Coq Require Import Derive.
+From NeuralNetInterp.Util Require Import ValueExtraction.
+From NeuralNetInterp.Torch Require Import Tensor.Instances.
+From NeuralNetInterp.MaxOfTwoNumbersSimpler Require Import Model Model.ExtraComputations.
+From NeuralNetInterp.MaxOfTwoNumbersSimpler.Computed Require Import AllLogits.
+
+Time #[local] Definition pre_logit_delta := logit_delta_float_gen (all_tokens (use_checkpoint:=false)) all_tokens_logits.
+Time #[local] Definition logit_delta_value := vm_compute pre_logit_delta.
+
+Time Definition logit_delta := (*Eval native_compute in pre *)Eval hnf in extract logit_delta_value.
+#[local] Strategy -100 [pre_logit_delta].
+Time Definition logit_delta_eq : logit_delta = ltac:(let v := eval cbv delta [pre_logit_delta] in pre_logit_delta in exact v) := extract_eq logit_delta_value.
