theories/MaxOfTwoNumbersSimpler/Model/ExtraComputations.v
@@ -1,4 +1,5 @@
 From NeuralNetInterp.TransformerLens Require Import HookedTransformer.Module.ExtraComputations.
+From NeuralNetInterp.TrainingComputations Require Import interp_max_utils.
 From NeuralNetInterp.MaxOfTwoNumbersSimpler Require Import Parameters Model.
 
-Module Export Model := ModelComputations cfg Model.
+Module Export Model := ExtraComputations.ModelComputations cfg Model <+ interp_max_utils.ModelComputations cfg Model.
