theories/MaxOfTwoNumbersSimpler/Model/ExtraComputations/Instances.v
@@ -1,0 +1,17 @@
+From Coq Require Import Morphisms RelationClasses RelationPairs.
+From NeuralNetInterp.Util Require Import Default SolveProperEqRel Option.
+From NeuralNetInterp.Util.Tactics Require Import Head DestructHead.
+From NeuralNetInterp.Util.List.Instances Require Import Forall2 Forall2.Map.
+From NeuralNetInterp.Torch Require Import Tensor Tensor.Instances Slicing Slicing.Instances.
+From NeuralNetInterp.TransformerLens Require Import HookedTransformer HookedTransformer.Instances HookedTransformer.Module.Instances.
+From NeuralNetInterp.TrainingComputations.interp_max_utils Require Import Instances.
+From NeuralNetInterp.MaxOfTwoNumbersSimpler Require Import Model.
+From NeuralNetInterp.MaxOfTwoNumbersSimpler.Model Require Import ExtraComputations Instances.
+Import Dependent.ProperNotations Dependent.RelationPairsNotations.
+
+Module Model.
+  Export ExtraComputations.Model.
+  Export Instances.Model.
+  Include ModelComputationsInstances cfg Model.Model Instances.Model ExtraComputations.Model.
+End Model.
+Export (hints) Model.
