theories/TrainingComputations/interp_max_utils/Instances.v
@@ -1,0 +1,42 @@
+From Coq Require Import Morphisms RelationClasses RelationPairs Relation_Definitions.
+From Coq Require Vector.
+From Coq.Structures Require Import Equalities.
+From Coq Require Import Floats Uint63 ZArith NArith.
+From NeuralNetInterp.Util.Tactics Require Import BreakMatch DestructHead.
+From NeuralNetInterp.Util Require Import Default SolveProperEqRel Option Pointed.
+From NeuralNetInterp.Util.Arith Require Import Classes Instances.
+From NeuralNetInterp.Util.List.Instances Require Import Forall2 Forall2.Map.
+From NeuralNetInterp.Torch Require Import Tensor Tensor.Instances Slicing Slicing.Instances.
+From NeuralNetInterp.TransformerLens Require Import HookedTransformer.
+From NeuralNetInterp.TransformerLens.HookedTransformer Require Import Config Instances Module Module.Instances.
+From NeuralNetInterp.TrainingComputations Require Import interp_max_utils.
+Import Dependent.ProperNotations Dependent.RelationPairsNotations.
+Import Instances.Truncating Instances.Uint63.
+#[local] Open Scope tensor_scope.
+#[local] Open Scope core_scope.
+
+Module ModelComputationsInstances (cfg : Config) (Import Model : ModelSig cfg) (Import ModelInstances : ModelInstancesSig cfg Model) (Import ModelComputations : ModelComputationsSig cfg Model).
+  Import (hints) cfg.
+
+  #[export] Instance logit_delta_Proper_dep
+    : Dependent.Proper
+        ((Dependent.const eq ==> Dependent.idR)
+           ==> (Dependent.idR ==> Dependent.idR ==> Dependent.idR)
+           ==> (Dependent.idR ==> Dependent.idR ==> Dependent.idR)
+           ==> (Dependent.idR ==> Dependent.idR ==> Dependent.idR)
+           ==> Dependent.const (fun _ _ => True)
+           ==> Dependent.const Tensor.eqf
+           ==> Tensor.eqfR
+           ==> Dependent.idR)
+        (@logit_delta).
+  Proof.
+    cbv [logit_delta]; repeat intro;
+      repeat lazymatch goal with
+        | [ H : (?x =? ?y) = true, H' : (?x =? ?y') = false |- ?G ]
+          => exfalso; cut (y = y');
+             [ revert H H'; generalize x y y'; clear; intros; subst; congruence
+             | clear H H'; now HookedTransformer.t ]
+        | _ => HookedTransformer.t_step
+        end.
+  Qed.
+End ModelComputationsInstances.
